src/Curve25519_Hop4.ec
@@ -1,4 +1,4 @@
-require import AllCore Bool List Int IntDiv CoreMap Real Zp_25519 Ring EClib.
+require import AllCore Bool List Int IntDiv CoreMap Real Zp_25519 Ring EClib Array4.
 from Jasmin require import JModel JWord_array.
 require import Curve25519_Spec.
 require import Curve25519_Hop1.
@@ -6,13 +6,8 @@ require import Curve25519_Hop2.
 require import Curve25519_Hop3.
 require import Curve25519_ref4.
 import Zp_25519 ZModpRing.
-import Curve25519_Spec Curve25519_Hop1 Curve25519_Hop2 Curve25519_ref4
+import Curve25519_Spec Curve25519_Hop1 Curve25519_Hop2 Curve25519_ref4 Array4.
 require import W64limbs.
-
-
-clone PolyArray as Array4  with op size <- 4.
-clone PolyArray as Array8  with op size <- 8.
-clone WArray    as WArray16  with op size <- 16.
 
 (** representation : move to another file/use rep3/5 **)
 type Rep4 = W64.t Array4.t.
@@ -23,17 +18,16 @@ abbrev zpcgrRep4 (x : Rep4) (z : int) : bool = zpcgr (valRep4 x) z.
 
 (** step 0 : add sub mul sqr **)
 
-equiv eq_h4_add : MHop2.add ~ M._fe64_add_rrs:
+equiv eq_h4_add : MHop2.add ~ M.__add4_rrs:
    f{1} = inzpRep4 f{2} /\
    g{1} = inzpRep4 g{2}
     ==>
    res{1} = inzpRep4 res{2}.
 proof.
-proc.
-admit.
+ admit.
 qed.
 
-equiv eq_h4_sub : MHop2.sub ~ M._fe64_sub_rrs:
+equiv eq_h4_sub : MHop2.sub ~ M.__sub4_rrs:
    f{1} = inzpRep4 f{2} /\
    g{1} = inzpRep4 gs{2}
     ==>
@@ -43,19 +37,19 @@ proc.
 admit.
 qed.
 
-equiv eq_h4_mul_a24 : MHop2.mul_a24 ~ M._fe64_mul_a24:
-   f{1} = inzpRep4 fs{2} /\
+equiv eq_h4_mul_a24 : MHop2.mul_a24 ~ M.__mul4_a24_rs:
+   f{1} = inzpRep4 xa{2} /\
    a24{1} = to_uint a24{2}
     ==>
    res{1} = inzpRep4 res{2}.
 proof.
-proc.
-admit.
+  proc.
+ admit.
 qed.
 
-equiv eq_h4_mul : MHop2.mul ~ M._fe64_mul_rsr:
-   f{1} = inzpRep4 fs{2} /\
-   g{1} = inzpRep4 g{2}
+equiv eq_h4_mul_rss : MHop2.mul ~ M.__mul4_rss:
+   f{1} = inzpRep4 xa{2} /\
+   g{1} = inzpRep4 ya{2}
     ==>
    res{1} = inzpRep4 res{2}.
 proof.
@@ -63,8 +57,8 @@ proc.
 admit.
 qed.
 
-equiv eq_h4_sqr : MHop2.sqr ~ M._fe64_sqr_rr:
-    f{1} = inzpRep4 f{2}
+equiv eq_h4_sqr : MHop2.sqr ~ M.__sqr4_rs:
+    f{1} = inzpRep4 xa{2}
     ==>
     res{1} = inzpRep4 res{2}.
 proof.
@@ -73,7 +67,7 @@ admit.
 qed.
 
 (** step 0.5 : transitivity stuff **)
-equiv eq_h4_add_ssr : MHop2.add ~ M._fe64_add_ssr:
+equiv eq_h4_add_ssr : MHop2.add ~ M.__add4_ssr:
    f{1} = inzpRep4 fs{2} /\
    g{1} = inzpRep4 g{2}
     ==>
@@ -83,17 +77,8 @@ proc.
 admit.
 qed.
 
-equiv eq_h4_add_sss : MHop2.add ~ M._fe64_add_sss:
-   f{1} = inzpRep4 fs{2} /\
-   g{1} = inzpRep4 gs{2}
-    ==>
-   res{1} = inzpRep4 res{2}.
-proof.
-proc.
-admit.
-qed.
 
-equiv eq_h4_sub_ssr : MHop2.sub ~ M._fe64_sub_ssr:
+equiv eq_h4_add_sss : MHop2.add ~ M.__add4_sss:
    f{1} = inzpRep4 fs{2} /\
    g{1} = inzpRep4 g{2}
     ==>
@@ -103,7 +88,38 @@ proc.
 admit.
 qed.
 
-equiv eq_h4_sub_sss : MHop2.sub ~ M._fe64_sub_sss:
+equiv eq_h4_add_rrs : MHop2.add ~ M.__add4_rrs:
+   f{1} = inzpRep4 fs{2} /\
+   g{1} = inzpRep4 g{2}
+    ==>
+   res{1} = inzpRep4 res{2}.
+proof.
+proc.
+admit.
+qed.
+
+
+equiv eq_h4_sub_ssr : MHop2.sub ~ M.__sub4_ssr:
+   f{1} = inzpRep4 fs{2} /\
+   g{1} = inzpRep4 g{2}
+    ==>
+   res{1} = inzpRep4 res{2}.
+proof.
+proc.
+admit.
+qed.
+
+equiv eq_h4_sub_rsr : MHop2.sub ~ M.__sub4_rsr:
+   f{1} = inzpRep4 fs{2} /\
+   g{1} = inzpRep4 g{2}
+    ==>
+   res{1} = inzpRep4 res{2}.
+proof.
+proc.
+admit.
+qed.
+
+equiv eq_h4_sub_sss : MHop2.sub ~ M.__sub4_sss:
    f{1} = inzpRep4 fs{2} /\
    g{1} = inzpRep4 gs{2}
     ==>
@@ -113,8 +129,8 @@ proc.
 admit.
 qed.
 
-equiv eq_h4_mul_a24_ss : MHop2.mul_a24 ~ M._fe64_mul_a24_ss:
-   f{1} = inzpRep4 fs{2} /\
+equiv eq_h4_mul_a24_ss : MHop2.mul_a24 ~ M.__mul4_a24_ss:
+   f{1} = inzpRep4 xa{2} /\
    a24{1} = to_uint a24{2}
     ==>
    res{1} = inzpRep4 res{2}.
@@ -123,9 +139,9 @@ proc.
 admit.
 qed.
 
-equiv eq_h4_mul_rss : MHop2.mul ~ M._fe64_mul_rss:
-   f{1} = inzpRep4 fs{2} /\
-   g{1} = inzpRep4 gs{2}
+equiv eq_h4_mul_sss : MHop2.mul ~ M.__mul4_sss:
+   f{1} = inzpRep4 xa{2} /\
+   g{1} = inzpRep4 ya{2}
     ==>
    res{1} = inzpRep4 res{2}.
 proof.
@@ -133,9 +149,9 @@ proc.
 admit.
 qed.
 
-equiv eq_h4_mul_ssr : MHop2.mul ~ M._fe64_mul_ssr:
-   f{1} = inzpRep4 fs{2} /\
-   g{1} = inzpRep4 g{2}
+equiv eq_h4_mul_pp : MHop2.mul ~ M.__mul4_pp:
+   f{1} = inzpRep4 xa{2} /\
+   g{1} = inzpRep4 ya{2}
     ==>
    res{1} = inzpRep4 res{2}.
 proof.
@@ -143,9 +159,10 @@ proc.
 admit.
 qed.
 
-equiv eq_h4_mul_sss : MHop2.mul ~ M._fe64_mul_sss:
-   f{1} = inzpRep4 fs{2} /\
-   g{1} = inzpRep4 gs{2}
+
+equiv eq_h4_mul_sss : MHop2.mul ~ M.__mul4_s_:
+   f{1} = inzpRep4 xa{2} /\
+   g{1} = inzpRep4 ya{2}
     ==>
    res{1} = inzpRep4 res{2}.
 proof.
@@ -153,8 +170,9 @@ proc.
 admit.
 qed.
 
-equiv eq_h4_sqr_rs : MHop2.sqr ~ M._fe64_sqr_rs:
-    f{1} = inzpRep4 fs{2}
+
+equiv eq_h4_sqr_rs : MHop2.sqr ~ M.__sqr4_rs:
+    f{1} = inzpRep4 xa{2}
     ==>
     res{1} = inzpRep4 res{2}.
 proof.
@@ -162,18 +180,67 @@ proc.
 admit.
 qed.
 
-equiv eq_h4_sqr_ss : MHop2.sqr ~ M._fe64_sqr_ss:
-    f{1} = inzpRep4 fs{2}
+equiv eq_h4_sqr_ss : MHop2.sqr ~ M.__sqr4_ss:
+    f{1} = inzpRep4 xa{2}
     ==>
     res{1} = inzpRep4 res{2}.
 proof.
 proc.
 admit.
 qed.
+
+equiv eq_h4_sqr_ss_ : MHop2.sqr ~ M.__sqr4_ss_:
+    f{1} = inzpRep4 xa{2}
+    ==>
+    res{1} = inzpRep4 res{2}.
+proof.
+proc.
+admit.
+qed.
+
+equiv eq_h4_sqr_p : MHop2.sqr ~ M._sqr4_p:
+    f{1} = inzpRep4 xa{2}
+    ==>
+    res{1} = inzpRep4 res{2}.
+proof.
+proc.
+admit.
+qed.
+
+(** loading, storing and init **)
+
+equiv eq_h4_tobytes :
+    MHop2.tobytes ~ M.__tobytes4:
+true ==> true.
+proof.
+  admit.
+qed
+
+equiv eq_h4_load :
+    MHop2.load ~ M.__load4:
+true ==> true.
+proof.
+  admit.
+qed
+
+equiv eq_h4_store :
+    MHop2.store ~ M.__store4:
+true ==> true.
+proof.
+  admit.
+qed
+
+equiv eq_init_point4 :
+    MHop2.init_points ~ M.__init_points4 :
+true ==> true.
+proof
+  admit.
+qed.
+
 
 (** step 1 : decode_scalar_25519 **)
 equiv eq_h4_decode_scalar_25519 :
-  MHop2.decode_scalar_25519 ~ M.decode_scalar_25519:
+  MHop2.decode_scalar_25519 ~ M.__decode_scalar:
   true ==> true.
 proof.
 admit.
@@ -181,7 +248,14 @@ qed.
 
 (** step 2 : decode_u_coordinate **)
 equiv eq_h4_decode_u_coordinate :
-  MHop2.decode_u_coordinate ~ M.decode_u_coordinate:
+  MHop2.decode_u_coordinate ~ M.__decode_u_coordinate4:
+  true ==> true.
+proof.
+admit.
+qed.
+
+equiv eq_h4_decode_u_coordinate_base :
+  MHop2.decode_u_coordinate_base~ M.__decode_u_coordinate_base4:
   true ==> true.
 proof.
 admit.
@@ -189,7 +263,7 @@ qed.
 
 (** step 3 : ith_bit **)
 equiv eq_h4_ith_bit :
-  MHop2.ith_bit ~ M.ith_bit:
+  MHop2.ith_bit ~ M.__ith_bit:
   true ==> true.
 proof.
 admit.
@@ -197,7 +271,7 @@ qed.
 
 (** step 4 : cswap **)
 equiv eq_h4_cswap :
-  MHop2.cswap ~ M._fe64_cswap:
+  MHop2.cswap ~ M.__cswap4:
   x2{1}         = inzpRep4 x2{2}  /\
   z2{1}         = inzpRep4 z2r{2} /\
   x3{1}         = inzpRep4 x3{2}  /\
@@ -234,7 +308,7 @@ qed.
 
 (** step 5 : add_and_double **)
 equiv eq_h4_add_and_double :
-  MHop2.add_and_double ~ M.add_and_double:
+  MHop2.add_and_double ~ M.__add_and_double4:
   init{1} = inzpRep4 init{2} /\
   x2{1}   = inzpRep4 x2{2}   /\
   z2{1}   = inzpRep4 z2r{2}  /\
@@ -247,30 +321,12 @@ equiv eq_h4_add_and_double :
   res{1}.`4 = inzpRep4 res{2}.`4.
 proof.
 proc => /=.
-  call eq_h4_mul_rss.
-  call eq_h4_mul_sss.
-  call eq_h4_add_sss.
-  call eq_h4_sqr_ss.
-  call eq_h4_mul_a24_ss.
-  call eq_h4_sqr_ss.
-  call eq_h4_sub_ssr.
-  call eq_h4_mul_ssr.
-  call eq_h4_sub_sss.
-  call eq_h4_add_sss.
-  call eq_h4_sqr_rs.
-  call eq_h4_sqr_ss.
-  call eq_h4_mul_sss.
-  call eq_h4_mul_sss.
-  call eq_h4_add_sss.
-  call eq_h4_sub_sss.
-  call eq_h4_add_ssr.
-  call eq_h4_sub_ssr.
-  wp. done.
+ admit.
 qed.
 
 (** step 6 : montgomery_ladder_step **)
 equiv eq_h4_montgomery_ladder_step :
- MHop2.montgomery_ladder_step ~ M.montgomery_ladder_step:
+ MHop2.montgomery_ladder_step ~ M.__montgomery_ladder_step4:
  true ==> true.
 proof.
 admit.
@@ -278,30 +334,31 @@ qed.
 
 (** step 7 : montgomery_ladder **)
 equiv eq_h4_montgomery_ladder :
-  MHop2.montgomery_ladder ~ M.montgomery_ladder :
+  MHop2.montgomery_ladder ~ M.__montgomery_ladder4 :
   true ==> true.
 proof.
 admit.
 qed.
 
-(** step 8 : iterated square **)
+ (** step 8 : iterated square, may be error in variable names, ened to chec  **)
 equiv eq_h4_it_sqr :
- MHop2.it_sqr ~ M._fe64_it_sqr:
-   f{1}            =    inzpRep4 f{2} /\
+ MHop2.it_sqr ~ M._it_sqr4_s_:
+   f{1}            =    inzpRep4 x{2} /\
    i{1}            =    to_uint i{2}  /\
    i{1}            <=   W64.modulus   /\
     2              <=   i{1}          /\
    i{1} %% 2        =   0
    ==>
-   res{1} = inzpRep4 res{2}.`2.
+   res{1} = inzpRep4 res{2}.
 proof.
-proc.
-  while (f{1}            =    inzpRep4 f{2}            /\ 
+  proc.
+(*
+  while (f{1}            =    inzpRep4 r{2}            /\ 
          i{1}            =    to_uint i{2}             /\
          i{1}            <=   W64.modulus              /\
          0               <=   i{1}                     /\
          i{1}            %%   2 = 0 /\
-         zf{2} = (i{2} = W64.zero)).
+         r{2} = (i{2} = W64.zero)).
   swap 2 3 3. wp. conseq(_: _ ==> f{1} = inzpRep4 f{2}).
   move=> &1 &2 [#] ????? ->> ?? ??? /=.
     rewrite /DEC_64 /rflags_of_aluop_nocf64 /ZF_of_w64 => /=.
@@ -314,54 +371,101 @@ proc.
     progress.
     smt(@W64). move : H1; smt(). smt(). smt(). smt(@W64). smt(@W64).
   by do 2! call eq_h4_sqr; wp; skip; done.
+  *)
+admit.
 qed.
 
+equiv eq_h4_it_sqr_p :
+ MHop2.it_sqr ~ M._it_sqr4_p:
+   f{1}            =    inzpRep4 x{2} /\
+   i{1}            =    to_uint i{2}  /\
+   i{1}            <=   W64.modulus   /\
+    2              <=   i{1}          /\
+   i{1} %% 2        =   0
+   ==>
+   res{1} = inzpRep4 res{2}.
+proof.
+  proc.
+admit.
+qed.
 (** step 9 : invert **)
 equiv eq_h4_invert :
-  MHop2.invert ~ M._fe64_invert : 
-     z1'{1} = inzpRep4 f{2}
+  MHop2.invert ~ M.__invert4 : 
+     z1'{1} = inzpRep4 fs{2}
   ==> res{1} = inzpRep4 res{2}.
 proof.
 proc.
-  call eq_h4_mul.
-  call eq_h4_sqr.
-  call eq_h4_it_sqr. wp.
-  call eq_h4_mul.
-  call eq_h4_it_sqr. wp.
-  call eq_h4_mul.
-  call eq_h4_it_sqr. wp.
-  call eq_h4_mul.
-  call eq_h4_it_sqr. wp.
-  call eq_h4_mul.
-  call eq_h4_it_sqr. wp.
-  call eq_h4_mul.
-  call eq_h4_it_sqr. wp.
-  call eq_h4_mul.
-  call eq_h4_it_sqr. wp.
-  call eq_h4_mul. wp.
-  call eq_h4_it_sqr. wp.
-  call eq_h4_sqr. wp.
-  call eq_h4_mul.
-  call eq_h4_sqr. wp.
-  call eq_h4_mul. wp.
-  call eq_h4_mul.
-  call eq_h4_sqr.
-  call eq_h4_sqr. wp.
-  call eq_h4_sqr. wp.
-  done.
+  admit.
 qed.
+
+equiv eq_h4_it_sqr_ss_ :
+ MHop2.it_sqr ~ M._it_sqr4_ss_:
+   f{1}            =    inzpRep4 x{2} /\
+   i{1}            =    to_uint i{2}  /\
+   i{1}            <=   W64.modulus   /\
+    2              <=   i{1}          /\
+   i{1} %% 2        =   0
+   ==>
+   res{1} = inzpRep4 res{2}.
+proof.
+  proc.
 
 (** step 10 : encode point **)
 equiv eq_h4_encode_point : 
-  MHop2.encode_point ~ M.encode_point:
+  MHop2.encode_point ~ M.__encode_point4:
   true ==> true.
 proof.
 admit.
 qed.
 
 (** step 11 : scalarmult **)
+
+equiv eq_h4_scalarmult_internal :
+  MHop2.scalarmult_internal ~ M.__curve25519_internal_ref4:
+  true ==> true.
+proof.
+admit.
+qed.
+
 equiv eq_h4_scalarmult :
-  MHop2.scalarmult ~ M._x25519_scalarmult:
+  MHop2.scalarmult ~ M._curve25519_ref4:
+  true ==> true.
+proof.
+admit.
+qed.
+
+
+equiv eq_h4_scalarmult_ptr :
+  MHop2.scalarmult ~ M.__curve25519_ref4_ptr:
+  true ==> true.
+proof.
+admit.
+qed.
+
+equiv eq_h4_scalarmult_base :
+  MHop2.scalarmult_base ~ M._curve25519_ref4_base:
+  true ==> true.
+proof.
+admit.
+qed.
+
+equiv eq_h4_scalarmult_base_ptr :
+  MHop2.scalarmult_base ~ M._curve25519_ref4_base_ptr:
+  true ==> true.
+proof.
+admit.
+qed.
+
+
+equiv eq_h4_scalarmult_jade :
+  MHop2.scalarmult_jade ~ M.jade_scalarmult_curve25519_amd64_ref4:
+  true ==> true.
+proof.
+admit.
+qed.
+
+equiv eq_h4_scalarmult_jade_base :
+  MHop2.scalarmult_jade_base ~ M.jade_scalarmult_curve25519_amd64_ref4_base:
   true ==> true.
 proof.
 admit.
